# Bayesian Lasso

## Bayesian Interpretation

We can show that $\hat{\boldsymbol\beta}_{LASSO}$ has a Bayesian interpretation. In particular, we can show that is a Bayes estimator for $\boldsymbol\beta$ assuming a multivariate Normal likelihood for $\mathbf{y}$:
$$f(y\mid \boldsymbol\beta, \sigma^2)\sim N(\mathbf{X}\boldsymbol\beta, \sigma^2\mathbf{I}),$$
and an independent double exponential (aka Laplace) prior for $\boldsymbol\beta$: 
$$f(\beta_j) = \left(\frac{\lambda}{2} \right)\exp(-\lambda |\beta_j|)$$

## Posterior

The posterior distribution for $\boldsymbol\beta$ (assuming $\sigma^2 = 1$ for simplicity): 

$$\begin{aligned}
g(\boldsymbol\beta \mid y)&\propto f(y \mid \boldsymbol\beta, \sigma^2) f(\boldsymbol\beta)\\
&= f(y \mid \boldsymbol\beta) \prod_{i=1}^p f(\beta_j)\text{, by independence assumption}\\
&=(2\pi)^{-n/2}\exp\left(-\frac{1}{2}(\mathbf{y} - \mathbf{X}\boldsymbol\beta)^\top (\mathbf{y} - \mathbf{X}\boldsymbol\beta) \right) \left(\frac{\lambda}{2}\right)^p \exp\left(-\lambda\sum_{j=1}^p |\beta_j|)\right)\\
&\propto\exp\left(-\frac{1}{2}(\mathbf{y} - \mathbf{X}\boldsymbol\beta)^\top (\mathbf{y} - \mathbf{X}\boldsymbol\beta) \right) \exp\left(-\lambda\sum_{j=1}^p |\beta_j|)\right)\\
&=\exp\left(-\frac{1}{2}(\mathbf{y} - \mathbf{X}\boldsymbol\beta)^\top (\mathbf{y} - \mathbf{X}\boldsymbol\beta)-\lambda\sum_{j=1}^p |\beta_j|)\right)
\end{aligned}$$

## Posterior Mode

Maximizing the posterior distribution, or minimizing the $-\log$ posterior, leads to $\beta_{LASSO}$.

$$\begin{aligned}\\
&\arg\max\text{ }\exp\left(-\frac{1}{2}(\mathbf{y} - \mathbf{X}\boldsymbol\beta)^\top (\mathbf{y} - \mathbf{X}\boldsymbol\beta)-\lambda\sum_{j=1}^p |\beta_j|)\right)\\
=\text{ }&\arg\max\text{ }-\frac{1}{2}(\mathbf{y} - \mathbf{X}\boldsymbol\beta)^\top (\mathbf{y} - \mathbf{X}\boldsymbol\beta)-\lambda\sum_{j=1}^p |\beta_j|\\
=\text{ }&\arg\min\text{ }\frac{1}{2}(\mathbf{y} - \mathbf{X}\boldsymbol\beta)^\top (\mathbf{y} - \mathbf{X}\boldsymbol\beta)+\lambda\sum_{j=1}^p |\beta_j|\\
=\text{ }&\arg\min\text{ -log posterior}\\
\end{aligned}$$

$$\begin{aligned}
\arg\min\text{ -log posterior}
&=\arg\min-\log(\exp\left(-\frac{1}{2}(\mathbf{y} - \mathbf{X}\boldsymbol\beta)^\top (\mathbf{y} - \mathbf{X}\boldsymbol\beta)-\lambda\sum_{j=1}^p |\beta_j|)\right))\\
&=\arg\min-\left(-\frac{1}{2}(\mathbf{y} - \mathbf{X}\boldsymbol\beta)^\top (\mathbf{y} - \mathbf{X}\boldsymbol\beta)-\lambda\sum_{j=1}^p |\beta_j|)\right)\\
&=\arg\min\frac{1}{2}(\mathbf{y} - \mathbf{X}\boldsymbol\beta)^\top (\mathbf{y} - \mathbf{X}\boldsymbol\beta)+\lambda\sum_{j=1}^p |\beta_j|\\
&=\beta_{LASSO}\text{, by definition}
\end{aligned}$$